isabelle/Semantics.thy
@@ -287,6 +287,8 @@ datatype Value = AvailableMoney AccountId Token
                | NegValue Value
                | AddValue Value Value
                | SubValue Value Value
+               | MulValue Value Value
+               | DivValue Value Value
                | ChoiceValue ChoiceId Value
                | SlotIntervalStart
                | SlotIntervalEnd
@@ -374,6 +376,10 @@ fun  evalValue :: "Environment \<Rightarrow> State \<Rightarrow> Value \<Rightar
     evalValue env state lhs + evalValue env state rhs" |
 "evalValue env state (SubValue lhs rhs) =
     evalValue env state lhs - evalValue env state rhs" |
+"evalValue env state (MulValue lhs rhs) =
+    evalValue env state lhs * evalValue env state rhs" |
+"evalValue env state (DivValue lhs rhs) =
+    (evalValue env state lhs) div (evalValue env state rhs)" |
 "evalValue env state (ChoiceValue choId defVal) =
     findWithDefault (evalValue env state defVal) choId (choices state)" |
 "evalValue env state (SlotIntervalStart) = fst (slotInterval env)" |
@@ -410,6 +416,10 @@ lemma evalDoubleNegValue :
 
 lemma evalNegValue :
   "evalValue env sta (AddValue x (NegValue x)) = 0"
+  by auto
+
+lemma evalMulValue :
+  "evalValue env sta (MulValue x (Constant 0)) = 0"
   by auto
 
 lemma evalSubValue :
